\let\negmedspace\undefined
\let\negthickspace\undefined
\documentclass[journal,12pt,twocolumn]{IEEEtran}
\usepackage{cite}
\usepackage{amsmath,amssymb,amsfonts,amsthm}
\usepackage{algorithmic}
\usepackage{graphicx}
\usepackage{textcomp}
\usepackage{xcolor}
\usepackage{txfonts}
\usepackage{listings}
\usepackage{enumitem}
\usepackage{mathtools}
\usepackage{gensymb}
\usepackage{comment}
\usepackage[breaklinks=true]{hyperref}
\usepackage{tkz-euclide} 
\usepackage{listings}
\usepackage{gvv}                                        
\def\inputGnumericTable{}                                 
\usepackage[latin1]{inputenc}                                
\usepackage{color}                                            
\usepackage{array}                                            
\usepackage{longtable}                                       
\usepackage{calc}                                             
\usepackage{multirow}                                         
\usepackage{hhline}                                           
\usepackage{ifthen}                                           
\usepackage{lscape}

\newtheorem{theorem}{Theorem}[section]
\newtheorem{problem}{Problem}
\newtheorem{proposition}{Proposition}[section]
\newtheorem{lemma}{Lemma}[section]
\newtheorem{corollary}[theorem]{Corollary}
\newtheorem{example}{Example}[section]
\newtheorem{definition}[problem]{Definition}
\newcommand{\BEQA}{\begin{eqnarray}}
\newcommand{\EEQA}{\end{eqnarray}}
\newcommand{\define}{\stackrel{\triangle}{=}}
\theoremstyle{remark}
\newtheorem{rem}{Remark}
\usepackage{circuitikz}
\begin{document}

\bibliographystyle{IEEEtran}
\vspace{3cm}

\title{GATE-2022, BM-37}
\author{EE23BTECH11033- JASWANTH KILLANA}
\maketitle
\newpage
\bigskip

\renewcommand{\thefigure}{\theenumi}
\renewcommand{\thetable}{\theenumi}
Question: Solution of the differential equation $\frac{dy}{dx}-y=cos\brak{x}$ is
\begin{align}
\brak{A}\quad y&=\frac{sin\brak{x}-cos\brak{x}}{2}+ce^x\\
\brak{B}\quad y&=\frac{sin\brak{x}+cos\brak{x}}{2}+ce^x\\
\brak{C}\quad y&=\frac{sin\brak{x}+cos\brak{x}}{2}+ce^{-x}\\
\brak{D}\quad y&=\frac{sin\brak{x}-cos\brak{x}}{2}+ce^{-x}
\end{align}
Solution:\begin{align}
\frac{dy}{dx}-y&=cos\brak{x}
\end{align}
Apply laplace transform
\begin{align}
\mathcal{L}\brak{\frac{dy}{dx}}-\mathcal{L}\brak{y}&=\mathcal{L}\brak{{cos\brak{x}}}
\end{align}
\begin{table}[!ht]
 \centering
  \input{tables\table1.tex}
   \caption{transformation}
   \end{table}
\begin{align}
\implies sY\brak{s}-y\brak{0}-Y\brak{s}&=\frac{s}{s^{2}+1}\\
Y\brak{s}\brak{s-1}&=y\brak{0}+\frac{s}{s^{2}+1}\\
Y\brak{s}&=\frac{s+y\brak{0}\brak{s^{2}+1}}{\brak{s-1}\brak{s^{2}+1}}\\
Y\brak{s}&=\frac{A}{s-1}+\frac{Bs+C}{s^2+1}\\
A&=y\brak{0},B=\frac{-1}{2},c=\frac{1}{2}\\
\implies Y\brak{s}&=\frac{y\brak{0}}{s-1}+\frac{-s+1}{2\brak{s^2+1}}
\end{align}
apply inverse laplace transform
\begin{align}
\mathcal{L^-}\brak{Y\brak{s}}&=\mathcal{L^-}\brak{\frac{y\brak{0}}{s-1}}+\mathcal{L^-}\brak{\frac{-s+1}{2\brak{s^2+1}}}\\
y\brak{x}&=y\brak{0}e^x+\frac{sin\brak{x}-cos\brak{x}}{2}
\end{align}
according to options 
\begin{align}
 y\brak{0}&=c\\
 \implies y&=\frac{sin\brak{x}-cos\brak{x}}{2}+ce^x
\end{align}
Option A is correct
\end{document}
